Cedille.lean
@@ -1,4 +1,5 @@
 
 import Cedille.Def
 import Cedille.Lemma
+import Cedille.Classify
 import Cedille.Theorem
